more examples and lots of documentation in FStar.DM4F.Heap.ST.fst

examples/dm4free/FStar.DM4F.Heap.ST.fst
@@ -1,3 +1,12 @@
+(* A state monad with local state built using FStar.DM4F.Heap. 
+   
+   The very end of the file illustrates how recursion through the heap
+   is forbidden because of the universe constraints.
+
+   As such, in this model, storing stateful functions in the heap is
+   forbidden. However, storing non-stateful functions, e.g,. Tot or
+   Exception function in the heap is acceptable.
+*)
 module FStar.DM4F.Heap.ST
 open FStar.DM4F.Heap
 
@@ -23,6 +32,10 @@ let get (_:unit): st heap =
 let put (x: heap): st unit =
   fun _ -> (), x
 
+////////////////////////////////////////////////////////////////////////////////
+// Instruct F* to CPS and elaborate the terms above to build a new STATE effect
+////////////////////////////////////////////////////////////////////////////////
+
 reifiable reflectable new_effect_for_free {
   STATE : a:Type -> Effect
   with repr     = st
@@ -33,54 +46,109 @@ reifiable reflectable new_effect_for_free {
      ; put      = put
 }
 
-
 inline let lift_pure_state (a:Type) (wp:pure_wp a) (h:heap) (p:STATE.post a) = wp (fun a -> p (a, h))
 sub_effect PURE ~> STATE = lift_pure_state
 
+//ST is an abbreviation for STATE with pre- and post-conditions
+//    aka requires and ensures clauses
 effect ST (a:Type) (pre: STATE.pre) (post: heap -> a -> heap -> Type0) =
        STATE a (fun n0 p -> pre n0 /\ (forall a n1. pre n0 /\ post n0 a n1 ==> p (a, n1)))
 
-val alloc : #a:Type0 -> init:a -> ST (ref a)
+//STNull is an abbreviation for stateful computations with trivial pre/post
+effect STNull (a:Type0) = ST a (fun h -> True) (fun _ _ _ -> True)
+
+////////////////////////////////////////////////////////////////////////////////
+//Next, given the primive global state actions STATE.get and STATE.put, 
+//we implement local state operations for allocating, reading and writing refs
+////////////////////////////////////////////////////////////////////////////////
+
+(* Allocation *)
+let alloc (#a:Type) (init:a)
+    : ST (ref a)
   	 (requires (fun h -> True))
 	 (ensures (fun h0 r h1 ->
-	 	     h1 `contains_a_well_typed` r
-		  /\ ~ (h0 `contains` r)
-		  /\ sel h1 r == init
-		  /\ modifies Set.empty h0 h1))
-let alloc #a init =
-   let h0 = STATE.get () in
-   let r, h1 = alloc h0 init in
-   STATE.put h1;
-   r
+	 	    ~ (h0 `contains` r)          //the ref r is fresh
+		  /\ h1 `contains_a_well_typed` r //and is well-typed in h1
+		  /\ sel h1 r == init             //initialized to init
+		  /\ modifies Set.empty h0 h1))   //and no existing ref is modified
+    = let h0 = STATE.get () in
+      let r, h1 = alloc h0 init in
+      STATE.put h1;
+      r
 
-val read : #a:Type0 -> r:ref a -> ST a
+(* Reading, aka dereference *)
+let read (#a:Type) (r:ref a)
+    : ST a
   	 (requires (fun h -> h `contains_a_well_typed` r))
 	 (ensures (fun h0 v h1 ->
-		     h0 == h1
-           	  /\  h1 `contains_a_well_typed` r
-		  /\  sel h1 r == v))
-let read #a r =
-   let h0 = STATE.get () in
-   sel h0 r
+		     h0 == h1                         //heap does not change
+           	  /\  h1 `contains_a_well_typed` r       
+		  /\  sel h1 r == v))                  //returns the contents of r
+   = let h0 = STATE.get () in
+     sel h0 r
 let (!) = read
 
-val write : #a:Type0 -> r:ref a -> v:a -> ST unit
+(* Writing, aka assignment *)
+let write (#a:Type) (r:ref a) (v:a)
+    : ST unit
   	 (requires (fun h -> h `contains_a_well_typed` r))
 	 (ensures (fun h0 _ h1 ->
            	     h0 `contains_a_well_typed` r
- 		  /\  h1 `contains_a_well_typed` r
-		  /\  h1 == upd h0 r v))
-let write #a r v =
-   let h0 = STATE.get () in
-   STATE.put (upd h0 r v)
+ 		  /\  h1 `contains_a_well_typed` r     //the heap remains well-typed
+		  /\  h1 == upd h0 r v))               //and is updated at location r only
+    = let h0 = STATE.get () in
+      STATE.put (upd h0 r v)
 let op_Colon_Equals = write
 
-effect STNull (a:Type) = ST a (fun h -> True) (fun _ _ _ -> True)
+////////////////////////////////////////////////////////////////////////////////
+//A simple example using the local state operations
+////////////////////////////////////////////////////////////////////////////////
+let incr (r:ref int) 
+    :  ST unit
+	  (requires (fun h -> h `contains_a_well_typed` r))
+	  (ensures (fun h0 s h1 -> 
+			     h0 `contains_a_well_typed` r
+			   /\ modifies (Set.singleton r) h0 h1
+			   /\ sel h1 r = sel h0 r + 1))
+    = r := !r + 1
 
-(* Uncomment the last two lines to see the following error message:
-   .\FStar.DM4F.Heap.ST.fst(84,26-84,47) : Error
-   Expected expression of type "Type(0)";
-   got expression "(uu___:Prims.unit -> STNull (Prims.unit))" of type "Type((S 0))"
-#set-options "--print_universes"
-let bad (x:unit) = alloc #(unit -> STNull unit) (fun () -> ())
-*) 
+let copy_and_incr (r:ref int) 
+    :  ST (ref int)
+	  (requires (fun h -> h `contains_a_well_typed` r))
+	  (ensures (fun h0 s h1 -> 
+			     h0 `contains_a_well_typed` r
+			   /\ ~ (h0 `contains` s)
+			   /\ h1 `contains_a_well_typed` s
+			   /\ modifies (Set.singleton r) h0 h1
+			   /\ sel h1 r = sel h0 r + 1
+			   /\ sel h1 s = sel h0 r))
+    = let s = alloc !r in
+      incr r; 
+      s
+      
+////////////////////////////////////////////////////////////////////////////////
+//A safe higher-order example
+//     Storing non-heap reading functions in the heap is fine
+////////////////////////////////////////////////////////////////////////////////
+let alloc_addition_and_incr (r:ref int)
+    : ST (ref (int -> Tot int))
+         (requires (fun h -> h `contains_a_well_typed` r))
+	 (ensures (fun h0 s h1 -> 
+			     h0 `contains_a_well_typed` r
+			   /\ ~ (h0 `contains` s)
+			   /\ h1 `contains_a_well_typed` s
+			   /\ modifies (Set.singleton r) h0 h1
+			   /\ (forall y. sel h1 s y = sel h0 r + y)))
+    = let x = !r in
+      let s = alloc (fun y -> x + y) in
+      s
+
+////////////////////////////////////////////////////////////////////////////////
+//An unsafe higher-example, rightly rejected because of an universe inconsistency
+//Uncomment the last two lines below to see the following error message:
+//   .\FStar.DM4F.Heap.ST.fst(145,29-145,50) : Error
+//   Expected expression of type "Type(0)";
+//   got expression "(uu___:Prims.int -> STNull Prims.int)" of type "Type((S 0))"
+////////////////////////////////////////////////////////////////////////////////
+(* #set-options "--print_universes" *)
+(* let bad (r:ref int) = alloc #(unit -> STNull unit) (fun () -> incr r) *)
